\documentclass[12pt]{article}
\author{Emmett Hitz}
\usepackage{amsmath}
\title{Partial Fractions}
\begin{document}
\maketitle
  \section*{9) $\frac{14x-41}{x^2-5x+4}$}
  factor denominator
  $$\frac{14x-41}{x^2-5x+4}=\frac{14x-41}{(x-4)(x-1)}$$
  begin decomposing
  $$\ldots = \frac{n_1}{x-4}+\frac{n_2}{x-1}$$
  multiply both sides by the original denominator
  $$\ldots = n_1(x-1)+n_2(x-4)$$
  $$14x-41=n_1x-n_1+n_2x-4n_2$$
  set up matrix equations
  $$14=n_1+n_2$$
  $$-41=-n_1-4n_2$$
  $$
  \left(
    \begin{array}{cc|c}
      1 & 1 & 14 \\ 
      -1 & -4 & -41 
    \end{array}
  \right)
  $$
  rref
  $$
  \left(
    \begin{array}{cc|c}
      1 & 0 & 5 \\ 
      0 & 1 & 9 
    \end{array}
  \right)
  $$
  $$\ldots = \frac{5}{x-4}+\frac{9}{x-1}$$
  \section*{10) $\frac{48-8x}{x^3-8x^2+16x}$}
  factor
  $$\ldots=\frac{-8(x-6)}{x(x-4)^2}$$
  begin decomposing
  $$\ldots=\frac{n_1}{x}+\frac{n_2}{x-4}+\frac{n_3}{(x-4)^2}$$
  multiply both sides by the original denominator
  $$\ldots=n_1(x-4)^2+n_2x(x-4)+n_3x$$
  distribute
  $$0x^2-8x+48=n_1x^2-8n_1x+16n_1+n_2x^2-4n_2x+n_3x$$
  group by $x$ to set up matrix
  $$0=n_1+n_2$$
  $$-8=-8n_1-4n_2+n_3$$
  $$48=16n_1$$
  $$
  \left(
    \begin{array}{ccc|c}
      1 & 1 & 0 & 0 \\ 
      -8 & -4 & 1 & -8 \\ 
      16 & 0 & 0 & 48 
    \end{array}
  \right)
  $$
  rref
  $$
  \left(
    \begin{array}{ccc|c}
      1 & 0 & 0 & 3 \\ 
      0 & 1 & 0 & -3 \\ 
      0 & 0 & 1 & 4 
    \end{array}
  \right)
  $$
  $$\ldots=\frac{3}{x}+\frac{-3}{x-4}+\frac{4}{(x-4)^2}$$ \newpage
  \section*{11) $\frac{5x^2+7x+11}{x^3+4x^2+5x+20}$}
  factor
  $$\ldots=\frac{5x^2+7x+11}{(x+4)(x^2+5)}$$
  begin decomposing (note: $x^2+5$ is a special case)
  $$\ldots=\frac{n_1}{x+4}+\frac{n_2x+n_3}{x^2+5}$$
  multiply both sides by the original denominator
  $$\ldots=n_1(x^2+5)+(n_2x+n_3)(x+4)$$
  $$\ldots=n_1x^2+5n_1+n_2x^2+4n_2x+n_3x+4n_3$$
  group by $x$ to set up matrix equations
  $$5=n_1+n_2$$
  $$7=4n_2+n_3$$
  $$11=5n_1+4n_3$$
  $$
  \left(
    \begin{array}{ccc|c}
      1 & 1 & 0 & 5 \\ 
      0 & 4 & 1 & 7 \\ 
      5 & 0 & 4 & 11
    \end{array}
  \right)
  $$
  rref 
  $$
  \left(
    \begin{array}{ccc|c}
      1 & 0 & 0 & 3 \\ 
      0 & 1 & 0 & 2 \\ 
      0 & 0 & 1 & -1
    \end{array}
  \right)
  $$
  $$\ldots=\frac{3}{x+4}+\frac{2x-1}{x^2+5}$$ \newpage
  \section*{12) $\frac{6x^3-5x^2+14x-19}{(x^2+3)^3}$}
  already factored\\ \\ 
  check for special cases. begin decomposing. (hint: use binomial expansion)
  $$\ldots=\frac{n_1x}{(x^2+3)^3}+\frac{n_2x}{(x^2+3)^2}+\frac{n_3}{(x^2+3)^3}+\frac{n_4}{(x^2+3)^2}$$
  multiply both sides by the original denominator
  $$\ldots=n_1x+n_2x(x^2+3)+n_3+n_4(x^2+3)$$
  distribute
  $$\ldots=n_1x+n_2x^3+3n_2x+n_3+n_4x^2+3n_4$$
  group by x to set up matrix equations
  $$6=n_2$$
  $$-5=n_4$$
  $$14=n_1+3n_2$$
  $$-19=n_3+3n_4$$
  $$
  \left(
    \begin{array}{cccc|c}
      0 & 1 & 0 & 0 & 6 \\ 
      0 & 0 & 0 & 1 & -5 \\ 
      1 & 3 & 0 & 0 & 14 \\
      0 & 0 & 1 & 3 & -19
    \end{array}
  \right)
  $$
  rref
  $$
  \left(
    \begin{array}{cccc|c}
      1 & 0 & 0 & 0 & -4 \\ 
      0 & 1 & 0 & 0 & 6 \\
      0 & 0 & 1 & 0 & -4 \\
      0 & 0 & 0 & 1 & -5 \\ 
    \end{array}
  \right)
  $$
  $$\ldots=\frac{-4x}{(x^2+3)^3}+\frac{6x}{(x^2+3)^2}+\frac{-4}{(x^2+3)^3}+\frac{-5}{(x^2+3)^2}$$

\end{document}